Split low projection definitions + model
The two different definitions of low projection and two different models
discussed in (issue #1722)[https://github.com/project-oak/oak/issues/1722]
are both alive in the code up to some smaller theorems.

The code redundancy is not ideal at the moment, so if these are really
meant to stay alive forever, then that should be improved at some point.

experimental/ni_coq/vfiles/LowEqPS.v
@@ -6,9 +6,8 @@ From OakIFC Require Import
     Parameters
     GenericMap
     Lattice
-    State
     Events
-    ModelTypes.
+    State.
 
 From RecordUpdate Require Import RecordSet.
 Import RecordSetNotations.
@@ -30,6 +29,7 @@ able to see channels labeled "Bob", so _any_ pair of channels with this label
 are related even if their contents differ.
 *)
 
+Definition trace := list (state * event_l).
 
 (*============================================================================
 * Low Projections
@@ -40,7 +40,7 @@ Definition low_proj {A: Type} ell ( labeled_thing: @labeled A) :=
     match labeled_thing with
         | Labeled _ o ell' => if( ell' <<? ell ) 
             then labeled_thing
-            else Labeled A None ell' 
+            else Labeled A None top
     end.
     (* 
     Importantly, the label of the secret thing is NOT ell'
@@ -139,7 +139,7 @@ Definition state_low_eq := fun ell s1 s2 =>
     and discussion in PossibilisticNI.v
 *)
 
-Inductive trace_low_eq: @trace_low_eqT (state * (@labeled event)) :=
+Inductive trace_low_eq: level -> trace -> trace -> Prop :=
     | NilEQ ell: trace_low_eq ell [] []
     | AddBoth ell xs xe ys ye t1 t2:
         trace_low_eq ell t1 t2 ->
